\documentclass{article}
\usepackage{amsfonts,amssymb,amsmath}
\usepackage[margin=1in]{geometry}

\title{CSCI 301, Winter 2018\\Math Exercises \# 4}
\author{Thomas Jones-Moore}
\date{Due date:  Thursday, February 8, midnight.}

\newcommand{\nats}{\ensuremath{\mathbb{N}}}

\begin{document}

\maketitle

Prove each of the following by induction, for all $n\in\nats$.
You may use SymPy or other symbolic algebra package to simplify
algebraic expressions.

\begin{enumerate}
\item
  \[
 \sum_{i=1}^n i^2 = \frac{n(n+1)(2n+1)}{6}
  \] \\
  \begin{alignat*}{2}
   &= \frac{1(1+1)(2(1)+1)}{6}=\frac{6}{6}=1 \\
   &1^2=1 \\
   &1+2+...+k^2+(k+1)^2= \frac{(k+1)(k+2)(2(k+1)+1)}{6} \\
   & \frac{k(k+1)(2k+1)}{6}+(k^2+2k+1) =\frac{(k^2+3k+2)(2(k+1)+1)}{6}\\
   &= \frac{(k^2+k)(2k+1)}{6}+(k^2+2k+1) =\frac{(k^2+3k+2)(2k+3)}{6}\\
   & \frac{2k^3+k^2+2k^2+k+6k^2+12k+6}{6}=\frac{2k^3+3k^2+6k^2+9k+4k+6}{6} \\
   &\frac{2k^3+9k^2+13k+6}{6}=\frac{2k^3+9k^2+13k+6}{6}
  \end{alignat*}
\item
  \[
 \sum_{i=1}^n i(i+1) = \frac{n(n+1)(n+2)}{3}
  \] \\
  \begin{alignat*}{2}
  &= \frac{1(1+1)(1+2)}{3}=\frac{1(2)(3)}{3}=2 \\
  &2=1(1+1) \\
  &= \frac{(k+1)(k+2)(k+3)}{3}  \\
  &= \frac{(k^2+2k+k+2)(k+3)}{3} \\
  &= \frac{k^3+6k^2+11k+6}{3} \\
  &1+2+...+k(k+1)+((k+1)(k+2))= \frac{k^3+6k^2+11k+6}{3} \\
  &\frac{k(k+1)(k+2)}{3}+(k+1)(k+2)= \\
  &\frac{k(k+1)(k+2)}{3}+\frac{3k^2+9k+6}{3}= \\
  &\frac{(k^2+k)(k+2)+3k^2+9k+6}{3}= \\
  &\frac{k^3+6k^2+11k+6}{3}=\frac{k^3+6k^2+11k+6}{3}
  \end{alignat*}
\item
  \[
 \sum_{i=1}^n (8i-5) = 4n^2 - n
 \] \\
 \begin{alignat*}{2}
 &= 4(1^2)-1=4-1=3\\
 & 3=(8*1-5) \\
 &=4((k+1)^2)-(k+1)\\
 &= 4(k^2+2k+1)-k-1 \\
 &= 4k^2+8k+4-k-1 \\
 &1+2+..+(8k-5)+(8(k+1)-5)= 4k^2+7k+3 \\
 &4k^2-k+8k+3=4k^2+7k+3 \\
 &4k^2+7k+3=4k^2+7k+3
 \end{alignat*}
\item
  \[
  3\mid (5^{2n} -1)
  \] \\
  \begin{alignat*}{2}
  &= (5^{2*1}-1) \\
  &= (25-1)=24 \\
  & 24\mod 3=0\\
  &=(5^{2(k+1)}-1) \\
  &=(5^{2k+2}-1) \\
  &=5^2*5^{2k}-1
  \end{alignat*}
\item
  \[
  9\mid (4^{3n} + 8)
  \]\\
  \begin{alignat*}{2}
  &4^{3*1}+8=72\\
  &72\mod9=0\\
  &=4^{3(k+1)}+8\\
  &=4^{3k+3}+8\\
  &=4^3*4^3k+8
  \end{alignat*}
\end{enumerate}


\end{document}